conc nearly done

automata.v
@@ -53,18 +53,18 @@ Definition dfa_run := [fun w => dfa_run' (dfa_s0 A) w].
 (** Acceptance of w in x is defined as
    finality of the last state of a run of w on A
    starting in x. **)
-Fixpoint dfa_accept' x w :=
+Fixpoint dfa_accept x w :=
 match w with
   | [::] => dfa_fin A x
-  | a::w => dfa_accept' (dfa_step A x a) w
+  | a::w => dfa_accept (dfa_step A x a) w
 end.
 
 (** We define the language of the deterministic
    automaton, i.e. acceptance in the starting state. **)
-Definition dfa_lang := [fun w => dfa_accept' (dfa_s0 A) w].
+Definition dfa_lang := [fun w => dfa_accept (dfa_s0 A) w].
 
-(** A lemma that helps us avoid cumbersome unfolding of accept' **)
-Lemma dfa_accept'S x a w : dfa_accept' x (a::w) = dfa_accept' (dfa_step A x a) w.
+(** A lemma that helps us avoid cumbersome unfolding of accept **)
+Lemma dfa_acceptS x a w : dfa_accept x (a::w) = dfa_accept (dfa_step A x a) w.
 Proof. elim: w x a => [|b w IHw] x a //=. Qed.
 (** Same for run' **)
 Lemma dfa_run'S x a w : dfa_run' x (a::w) = (dfa_step A x a) :: dfa_run' (dfa_step A x a) w.
@@ -128,15 +128,15 @@ Section Acceptance.
 Variable A: nfa.
 
 (** Non-deterministic acceptance. **)
-Fixpoint nfa_accept' (x: state) w :=
+Fixpoint nfa_accept (x: state) w :=
 match w with
   | [::] => nfa_fin A x
-  | a::w => existsb y, (nfa_step A x a y) && nfa_accept' y w
+  | a::w => existsb y, (nfa_step A x a y) && nfa_accept y w
 end.
 
 (** We define the language of the non-deterministic
    automaton, i.e. acceptance in the starting state. **)
-Definition nfa_lang := [fun w => nfa_accept' (nfa_s0 A) w].
+Definition nfa_lang := [fun w => nfa_accept (nfa_s0 A) w].
 
 (** We define labeled paths over the non-deterministic step relation **)
 Fixpoint nfa_lpath x (xs : seq state) (w: word) {struct xs} :=
@@ -147,9 +147,9 @@ match xs,w with
 end.
 
 (** We proof that there is a path labeled with w induced
-   by nfa_accept' starting at x and ending in an accepting
+   by nfa_accept starting at x and ending in an accepting
    state. **)
-Lemma nfa_accept_lpath x w: nfa_accept' x w -> exists xs, nfa_lpath x xs w /\ nfa_fin A (last x xs).
+Lemma nfa_accept_lpath x w: nfa_accept x w -> exists xs, nfa_lpath x xs w /\ nfa_fin A (last x xs).
 Proof. elim: w x => [|a w IHw] x.
   by exists [::].
 move => /existsP [] y /andP [] H0 /IHw [xs [H1 H2]].
@@ -159,7 +159,7 @@ Qed.
 
 (** We proof that the existence of a path labeled with w
    implies the acceptance of w. **)
-Lemma nfa_lpath_accept x xs w: nfa_lpath x xs w -> nfa_fin A (last x xs) -> nfa_accept' x w.
+Lemma nfa_lpath_accept x xs w: nfa_lpath x xs w -> nfa_fin A (last x xs) -> nfa_accept x w.
 Proof. elim: w x xs => [|a w IHw] x xs.
   (* We destruct the path to ensure that it is empty. *)
   case: xs => [|y xs].
@@ -173,6 +173,24 @@ simpl. move => [] /andP [] H0 H1 H2.
 apply/existsP. exists y.
 rewrite H0 andTb.
 apply: IHw; by eassumption.
+Qed.
+
+(** Helpful facts **)
+Lemma nfa_accept_cat x w1 w2:
+  nfa_accept x (w1 ++ w2) <->
+  exists xs,
+    nfa_lpath x xs w1
+    && nfa_accept (last x xs) w2.
+Proof. split.
+  elim: w1 w2 x => [|a w1 IHw1] w2 x.
+    simpl. exists [::]. simpl. exact: H.
+  move/existsP => [] y /andP [] H0 /IHw1 [] ys /andP [] H1 H2.
+  exists (y::ys) => /=. by rewrite H0 H1 H2.
+elim: w1 w2 x => [|a w1 IHw1] w2 x; move => [] [|y ys] /andP [] H0 H1 //.
+move: H0 => /= /andP [] H2 H3. 
+apply/existsP. exists y. rewrite H2 => /=.
+apply: IHw1.
+exists ys. by rewrite H3 H1.
 Qed.
 
 End Acceptance.
@@ -206,7 +224,7 @@ Definition nfa_to_dfa :=
    accepts at least the language of the given automaton
    when starting in a set containing x. **)
 Lemma nfa_to_dfa_correct1 (x: state) w (X: powerset_state):
-  x \in X -> nfa_accept' A x w -> dfa_accept' nfa_to_dfa X w.
+  x \in X -> nfa_accept A x w -> dfa_accept nfa_to_dfa X w.
 Proof. move => H0.
   (* "->" *)
   elim: w X x H0 => [|a w IHw] X x H0.
@@ -234,7 +252,7 @@ Qed.
    representative state of that set in which the given automaton
    accepts w. **)
 Lemma nfa_to_dfa_correct2 (X: powerset_state) w:
-  dfa_accept' nfa_to_dfa X w -> existsb x, (x \in X) && nfa_accept' A x w.
+  dfa_accept nfa_to_dfa X w -> existsb x, (x \in X) && nfa_accept A x w.
 Proof. elim: w X => [|a w IHw] X.
   by [].
 move/IHw => /existsP [] y /andP [].
@@ -275,7 +293,7 @@ Definition dfa_to_nfa : nfa state :=
 
 (** We proof that dfa_to_nfa accepts the same language as
    the given automaton in any state. **)
-Lemma dfa_to_nfa_correct' x w : dfa_accept' A x w = nfa_accept' dfa_to_nfa x w.
+Lemma dfa_to_nfa_correct' x w : dfa_accept A x w = nfa_accept dfa_to_nfa x w.
 Proof. elim: w x => [|b w IHw] x.
   by [].
 simpl. rewrite IHw.
@@ -303,28 +321,29 @@ Variable A1: dfa state1.
 
 
 (** Complement automaton **)
-Section Complement.
   
 (** The only change needed is to negate the finality predicate. **)
-Definition fin_compl := [ fun x1 => ~~ fin1 x1 ].
+Definition fin_compl := [ fun x1 => ~~ dfa_fin A1 x1 ].
 (** We construct the resulting automaton. **)
 Definition dfa_compl :=
   dfaI
-  state1
-  (s0 A1)
-  fin_compl
-  step1.
+    state1
+    (dfa_s0 A1)
+    fin_compl
+    (dfa_step A1).
 
 (** We proof that the complement automaton accepts exactly
    the words not accepted by the original automaton. **)
-Lemma dfa_compl_correct' w q: accept' A1 q w = ~~ accept' Aut_not q w.
-Proof.
+Lemma dfa_compl_correct' w x: dfa_accept A1 x w = ~~ dfa_accept dfa_compl x w.
+Proof. elim: w x => [|a w IHw] x.  
   by apply/idP/negPn.
+simpl. by rewrite IHw.
 Qed.
 
+Lemma dfa_compl_correct w: dfa_lang A1 w = ~~ dfa_lang dfa_compl w.
+Proof. exact: dfa_compl_correct'. Qed.
 
-End Complement.
-
+  
 (** Operations on two automata. **)
 Section BinaryOps.
   
@@ -345,7 +364,7 @@ Definition dfa_disj :=
     step_disj.
 
 (** Correctness w.r.t. any state. **)
-Lemma dfa_disj_correct' w x1 x2 : dfa_accept' A1 x1 w || dfa_accept' A2 x2 w = dfa_accept' dfa_disj (x1, x2) w.
+Lemma dfa_disj_correct' w x1 x2 : dfa_accept A1 x1 w || dfa_accept A2 x2 w = dfa_accept dfa_disj (x1, x2) w.
 Proof. elim: w x1 x2 => [|a w IHw].
   by [].
 move => x1 x2. by exact: IHw.
@@ -367,7 +386,7 @@ Definition dfa_conj :=
 .
 
 (** Correctness w.r.t. any state. **)
-Lemma dfa_conj_correct' w x1 x2 : dfa_accept' A1 x1 w && dfa_accept' A2 x2 w = dfa_accept' dfa_conj (x1, x2) w.
+Lemma dfa_conj_correct' w x1 x2 : dfa_accept A1 x1 w && dfa_accept A2 x2 w = dfa_accept dfa_conj (x1, x2) w.
 Proof. elim: w x1 x2 => [|a w IHw].
   by [].
 move => x1 x2.
@@ -382,498 +401,122 @@ End BinaryOps.
 
 End DFAOps.
 
-
-
-End FA.
-
-
-
-
-(** Operations on up to two automata with the same alphabet **)
-Section Operators.
-Variable char: finType.
+(** Operations on non-deterministic automata. **)
+Section NFAOps.
 Variable state1 state2: finType.
-Variable s01: state1.
-Variable s02: state2.
-Variable fin1: pred state1.
-Variable fin2: pred state2.
-Variable step1: state1 -> char -> state1.
-Variable step2: state2 -> char -> state2.
+Variable A1: nfa state1.
+Variable A2: nfa state2.
 
-Variable A1: dfa char state1 s01 fin1 step1.
-Variable A2: dfa char state2 s02 fin2 step2.
+(** Concatenation of two non-deterministic automata. **)
 
+Definition state_conc : finType := sum_finType state1 state2.
 
-
-
-
-
-  
-
-
-
-(** Star automaton. **)
-Section Star.
-  
-(** We need to add a new state. **)
-Definition state_star' := option_finType state1.
-Definition s0_star' : state_star' := None.
-(** We only accept the empty state. **)
-Definition fin_star' := [ pred x | x == s0_star' ].
-(** The type of states in the star automaton. **)
-Definition state_star := state_det state_star'.
-(** We construct a non-functional relation which is 
-   the new transitions of the star automaton.
-   Whenever we enter a former final state, we
-   also enter the new starting state, thereby
-   ensuring acceptance. **)
-Definition step_rel_star : state_star' -> char -> pred state_star' :=
-  (fun x1 a =>
-    match x1 with
-      (** any old state **)
-      | Some x1 => [ pred x2 |
-                       (x2 == Some (step1 x1 a))
-                    || (fin1 (step1 x1 a) && (x2 == s0_star'))
-                   ]
-      (** the new state s0_sta **)
-      | s0_star' => [ pred x2 | x2 == Some (step1 s01 a) ]
-    end
-  ).
-(** We construct the star automaton. **)
-(** Definition Aut_star := to_dfa char state1 s01 fin_star' step_rel_star. **)
-Definition step_star := step_det char step_rel_star.
-Definition s0_star := s0_det state_star' s0_star'.
-Definition fin_star := fin_det state_star' fin_star'.
-Definition Aut_star := dfaI char (state_det state_star') s0_star fin_star step_star.
-
-(** Starting state correctness. **)
-Lemma Aut_star_s0 : s0_star s0_star'. by rewrite /s0_star /s0_det ffunE eq_refl. Qed.
-
-(** step_star_rel invariant. **)
-Lemma Aut_star_step_rel (X: state_star) a: fin_star (step_star X a) -> (step_star X a) s0_star'.
-Proof. simpl. move/existsP => [] x. by rewrite andbC => /andP [] /eqP ->. Qed.
-  
-(** We proof that the empty word is contained in the
-   language of the star automaton. **)
-Lemma Aut_star_correct0 : accept Aut_star [::].
-Proof. rewrite/accept/accept'/fin_star => /=. apply/existsP. exists s0_star'.
-by rewrite /s0_det ffunE eq_refl. Qed.
-
-(** We proof that all non-empty words accepted by the
-   original automaton are also accepted by the star
-   automaton.
-   Translating x to [pred x' | x'==x] gives us an
-   induction hypothesis which is too weak to prove
-   the statement. Therefore, we allow the star automaton
-   to start from any set of states containing x.
-   **)
-Lemma Aut_star_correctS (X: state_star) a w x :
-  X (Some x) -> accept' A1 x (a::w) -> accept' Aut_star X (a::w).
-Proof. elim: w a X x => [| b w IHw ] a X x H0.
-  move => /= H1. apply/existsP. exists s0_star'. rewrite ffunE eq_refl andbT.
-  apply/existsP. exists (Some x). rewrite H0 andTb /step_rel_star /=.
-  by rewrite H1 eq_refl.
-rewrite accept'S. apply: IHw. rewrite ffunE. apply/existsP. exists (Some x).
-by rewrite H0 andTb /step_rel_star /= eq_refl.
-Qed.
-
-(** We show that every accepting run of the
-   star automaton ends in a state Y s.t. Y s0_star'. **)
-Lemma Aut_star_end X w: accept' Aut_star X w -> last X (run' Aut_star X w) s0_star'.
-Proof. elim: w X => [|a w IHw] X.
-  by move => /= /existsP [] q /andP [] H0 /eqP <-.
-rewrite accept'S. by apply: IHw.
-Qed.
-
-(** We define the notion of a shortest, non-empty, accepting prefix **)
-Definition Aut_star_prefix (X: state_star) (w: word char) (n: nat) : bool :=
-      (n > 0) && (n <= size w) && (accept' Aut_star X (take n w)) &&
-  forallb n': ordinal n, (n' > 0) ==> ~~ accept' Aut_star X (take n' w).
- 
-(** We proof that there are no shorter prefixes than the shortest prefix. **)
-Definition Auf_star_prefix_shortest (X: state_star) (w: word char) (n: nat) :
-  Aut_star_prefix X w n -> forallb n' : 'I_n, ~~ Aut_star_prefix X w n'.
-Proof. move: w X. apply: last_ind => [| w b IHw ] X.
-  rewrite /Aut_star_prefix => /andP [] /andP [] /andP []. rewrite lt0n => H0.
-  rewrite leqn0 => H1. by move: H1 H0 => ->.
-rewrite /Aut_star_prefix => /andP [] /andP [] /andP [] H0 H1 H2 /forallP H3.
-apply/forallP => m. rewrite 3!negb_and. apply/orP. left.
-case_eq (nat_of_ord m == 0).
-  by move/eqP => ->.
-move/neq0_lt0n => H4. apply/orP. right.
-move: (H3 m) => /implyP. move => H5. apply: H5. by [].
-Defined.
-
-(** This, too. **)
-Lemma word_expand (w: word char) : 0 < (size w) -> exists a, w = rcons (take (size w).-1 w) a.
-Proof. move: w. apply: last_ind => [| w a IHw].
-  by [].
-move => H0. exists a.
-rewrite -cats1 takel_cat.
-  rewrite -cats1 size_cat. rewrite addn1. by rewrite take_size.
-by rewrite size_cat addn1.
-Qed.
-
-(** We proof that Aut_star_prefix is "transitive" regarding
-   additional suffixes. **)
-Lemma Aut_star_prefix_trans X w k m:
-k >= m -> Aut_star_prefix X (take k w) m -> Aut_star_prefix X w m.
-Proof. move: w m k. apply: last_ind => [|w b IHw] m k.
-  by [].
-move => H0.
-case_eq (k < size (rcons w b)) => H1.
-  rewrite -cats1 takel_cat.
-    move/andP => [] /andP [] /andP [] H2 H3 H4 /forallP H5.
-    (** we'll need this a few times: **)
-    have: m <= size w.
-      apply: leq_trans.
-        by apply H3.
-      exact: size_take_bound.
-    move => H6.
-    
-    rewrite /Aut_star_prefix. rewrite H2.
-    have: m <= size (w++ [::b]).
-      apply: leq_trans.
-          by apply H6.
-        rewrite cats1 size_rcons.
-        by apply: ltnW.
-      move => ->.
-    rewrite take_undersize in H4 => //.
-    rewrite takel_cat => //.
-    rewrite H4.
-    rewrite 2!andTb.
-    apply/forallP => n'.
-    rewrite takel_cat.
-      move: (H5 n').
-      rewrite take_undersize => //.
-      apply: leq_trans.
-        apply ltnW.
-        by apply (ltn_ord n').
-      by [].
-    apply: leq_trans.
-      apply ltnW.
-      by apply (ltn_ord n').
-    exact: H6.
-  move: H1.
-  rewrite size_rcons. by rewrite ltnS.
-move: (negbT H1). rewrite -leqNgt => H2.
-by rewrite take_oversize.
-Qed.
-
-(** We proof that there are no accepted prefixes < n if there is
-   no shortest, non-empty, accepting prefix < n **)
-Lemma Aut_star_prefix_none X w a n:
-  0 < n ->
-  (forallb m : 'I_(S n), (0 < m) ==> ~~ Aut_star_prefix X (rcons w a) m) -> ~~ accept' Aut_star X (take n (rcons w a)).
-Proof. elim: n X w a => [|n IHn] X w a;
-move => H0 /forallP H1.
-  by [].
-pose m := (@Ordinal n.+2 n.+1 (ltnSn n.+1)).
-have: n.+1 = nat_of_ord m. by []. move => H3.
-move: (H1 m) => /implyP H4.
-have: (0 < m). rewrite -H3. by [].
-move: (H4 H0).
-rewrite 3!negb_and. move/orP => [].
-  move/orP => [].
-    move/orP => [].
-      rewrite ltnNge. move/negbNE.
-      rewrite leq_eqVlt => /orP [].
-        rewrite -H3 => /eqP H5. by move : H5 H0 => ->.
-      by [].
-    rewrite leqNgt. move/negbNE. rewrite -{1}H3 => H5 H6.
-    apply/negbT. rewrite take_oversizeS.
-      apply/negbTE.
-      case_eq n => [|n'].
-        move => H7. rewrite H7 in H5. move: H5. rewrite ltnS. rewrite leqn0.
-        rewrite size_rcons. by [].
-      move => H7. rewrite -H7. apply IHn.
-        rewrite H7. by [].
-      apply/forallP. move => k. move: (ltn_ord k). move/leqW => H8.
-      pose k' := (@Ordinal n.+2 k H8).
-      have: nat_of_ord k' = k. by [].
-      move => <-. by apply H1.
-      exact: H5.
- 
-   move => H5 H6. rewrite H3. exact H5.
-rewrite -negb_exists_in. move/negbNE => /existsP [] k.
-move/andP => [] H5 H6 H7.
-move: (H4 H7). rewrite 3!negb_and. rewrite H7. rewrite orFb.
-  case_eq (m <= size (rcons w a)) => H8.
-    rewrite orFb.
-  move/orP => [].
-    by rewrite -H3. 
-  rewrite -negb_exists_in. move/negbNE => /existsP [].
-     
-Admitted.
-
-(** We proof that there is a shortest, non-empty, accepting prefix
-   for every non-empty word accept by the star automaton. **)
-Lemma Aut_star_shortest_prefix (X: state_star) (a: char) w:
-  accept' Aut_star X (rcons w a) ->
-  exists n,
-    Aut_star_prefix X (rcons w a) n.
-Proof.
-(** We use size_induction to get a helpful IH. **)
-move: w a X. apply: (size_induction size) => w IHw a X.
-case_eq (size w) => [|s] Hs.
-  rewrite (size0nil Hs).
-  move => H0. 
-  exists 1. apply/andP. split.
-    rewrite andTb. by exact: H0. 
-  apply/forallP => x. apply/implyP. move: (ltn_ord x).
-  rewrite leq_eqVlt => /andP [] /eqP H1.
-  (** this is a very convoluted way of proving that x=0. **)
-  case_eq (nat_of_ord x) => [|x'].
-    by [].
-  move/(f_equal S). rewrite H1. move/(f_equal predn). by [].
-
-(** We use word_expand to get separate prefix and the 1-suffix **)
-have: 0 < size w.
-  by rewrite Hs.
-move/word_expand => [] b Hw. rewrite Hw.
-move Ew: (take (size w).-1 w) => w'.
-move => H0.
-(** See if there already is a prefix: **)
-case_eq (existsb m : 'I_ (size (rcons (rcons w' b) a)), Aut_star_prefix X (rcons w' b) m).
-(** prefix. **)
-  move/existsP => [] m /andP [] /andP [] /andP [] H1 H2 H3 /forallP H4.
-  pose n:=nat_of_ord m.
-  exists n. apply/andP. split.
-    apply/andP. split.
-      apply/andP. split => //.
-      rewrite size_rcons.
-        move: H2. by exact: leqW.
-      rewrite -{}cats1. rewrite {1}(takel_cat H2). 
-      by exact: H3.
-  apply/forallP => k. apply/implyP => H5.
-  rewrite -cats1 takel_cat. move: H5. apply/implyP. by exact: H4.
-  apply: leq_trans. apply ltnW. apply ltn_ord. by [].
-
-(** no prefix. **)
-
-move/negbT. rewrite negb_exists => /forallP H1. exists (size (rcons (rcons w' b) a)).
-apply/andP. split.
-  apply/andP. split.
-    by rewrite size_rcons ltn0Sn ltnSn.
-  rewrite take_size. by exact: H0.
-apply/forallP => n'. apply/implyP => H2.
-move: (H1 n').
-(** We'll need this a few times. **)
-have: (n' <= size (rcons w' b)).
-    rewrite -{1}ltnS -(size_rcons (rcons w' b ) a).
-    exact: (ltn_ord n').
-move => H3.
-
-rewrite negb_and H2 => /orP [].
-  rewrite negb_and => /orP [].
-    rewrite negb_and => /orP [].
-      by [].
-    by rewrite H3. 
-  rewrite -(takel_cat H3 [::a]).
-  by rewrite cats1.
-
-rewrite negb_forall.
-rewrite negb_forall_in.
-move/existsP => [] m.
-(** take m w' would be the shortest, non-empty, accepting prefix
-   but there is no such prefix. **)
-move/andP => [] H4 /negbNE H5.
-Admitted.
-
-
-Lemma Aut_star_prefix_det w a n:
-  Aut_star_prefix s0_star (rcons w a) n ->  accept A1 (take n (rcons w a)).
-Proof. move: w a n. apply: last_ind => [|w b IHw] a n.
-  move => /andP [] /andP [] /andP [] H0 H1 H2 /forallP H3.
-  rewrite take_oversize /accept' in H2 => //.
-  rewrite /A_fin /fin_star /s0_star in H2.
-  move: H2 => /existsP [] y /andP [].
-  rewrite /run' ffunE => /existsP [] z.
-  rewrite ffunE => /andP [] /eqP ->.
-  rewrite /step_rel_star /fin_star' => /= /eqP ->. by [].
-
-move => /andP [] /andP [] /andP [] H0 H1 H2 /forallP H3.
-
-case_eq (n < size (rcons (rcons w b) a)).
-  rewrite size_rcons => H4.
-  have: n <= size (rcons w b). by []. move => H5.
-  move: H2. rewrite -cats1. rewrite takel_cat => //.
-  move => H2. apply: IHw.
-  rewrite /Aut_star_prefix H0 H5 H2 2!andTb.
-  apply/forallP. move => m.
-  move: (H3 m). rewrite -cats1 takel_cat.
-    by [].
-  apply: leq_trans.
-    eapply ltnW.
-    by eapply ltn_ord.
-  by [].
-
-Admitted.
-  
-End Star.
-
-(** Concatenation **)
-Section Concatenation.
-  
-Definition state_sum := sum_finType state1 state2.
-Definition state_sum_option := option_finType state_sum.
-
-Definition state1_conc (x1: state1) : state_sum. constructor. exact x1. Defined.
-Definition state2_conc (x2: state2) : state_sum. apply/inr. exact x2. Defined.
-Definition state_conc := state_det state_sum.
-Definition s0_conc : state_sum. constructor. exact: s01. Defined.
-
-Definition step_conc (x: state_sum) a (x': state_sum) := 
-match x with
-| inl x1 => 
-  match x' with
-  | inl x1' => step1 x1 a == x1'
-  | inr x2' => fin1 x1 && (step2 s02 a == x2')
-  end
-| inr x2 =>
-  match x' with
-  | inr x2' => step2 x2 a == x2'
-  | _ => false
-  end
+Definition step_conc x a y :=
+match x,y with
+  | inl x, inl y => nfa_step A1 x a y
+  | inl x, inr y => nfa_fin A1 x && nfa_step A2 (nfa_s0 A2) a y
+  | inr x, inr y => nfa_step A2 x a y
+  | inr x, inl y => false
 end.
 
-Definition fin_conc := [fun x : state_sum =>
+Definition fin_conc (x: state_conc) : bool :=
 match x with
-| inl x1 => fin1 x1 && fin2 s02
-| inr x2 => fin2 x2
-end ].
-Definition Aut_conc := to_dfa char state_sum (s0_conc) fin_conc step_conc. 
+  | inl x => nfa_fin A1 x && nfa_fin A2 (nfa_s0 A2)
+  | inr x => nfa_fin A2 x
+end.
 
-(** We define a relation (an order) on states. **)
-Definition state_conc_leq (q1' q2': state_conc) := forall q, q1' q -> q2' q.
+Definition s0_conc : state_conc := inl _ (nfa_s0 A1).
 
-Notation "q1' ===> q2'" := (state_conc_leq q1' q2') (at level 70).
+Definition nfa_conc : nfa state_conc :=
+  nfaI
+    state_conc
+    s0_conc
+    fin_conc
+    step_conc.
 
-(** We proof a few interesting properties of this relation. **)
-Lemma q_conc_leq_trans (q1' q2' q3': state_conc) : q1' ===> q2' -> q2' ===> q3' -> q1' ===> q3'.
-Proof. rewrite/state_conc_leq. move => H0 H1 q. by move/H0/H1. Qed.
-
-Lemma q_conc_leq_d_trans (q1' q2' : state_conc) a : 
-q1' ===> q2' -> step_det char step_conc q1' a ===> step_det char step_conc q2' a.
-Proof. move => H0 q. rewrite/step_det. rewrite 2!ffunE. 
-move/existsP => [] p /andP [] /H0 H1 H2. apply/existsP. exists p. 
-by rewrite H1 H2. Qed.
-
-Lemma Aut_conc_expand1 (q1' q2': state_conc) w:
-q1' ===> q2' ->
-accept' Aut_conc q1' w ->
-accept' Aut_conc q2' w.
-Proof. elim: w q1' q2' => [|a w IHw]. 
-  rewrite/accept'/fin_det => /= q1' q2' H. move/existsP => [] q /andP []. 
-  move => H0 H1. apply/existsP. move: (H q H0). exists (q). by rewrite H2 H1.
-move => q1' q2'. move/(@q_conc_leq_d_trans _ _ a). simpl. 
-by apply: IHw.
+Lemma nfa_conc_cont x xs w:
+  nfa_lpath A2 x xs w
+  -> nfa_lpath nfa_conc (inr _ x) (map (@inr state1 state2) xs) w.
+Proof. elim: xs x w => [|y xs IHxs] x w; case: w => [|a w] => //.
+simpl. by move/andP => [] -> /IHxs ->.
 Qed.
 
-(** We proof that the concatenation automaton accepts
-   all words of the first automaton if the second automaton
-   accepts the empty word. **)
-Lemma Aut_conc_correct1' q1 w1: 
-accept' A1 q1 w1 && accept A2 [::] 
--> accept' Aut_conc (finfun (fun q=> q == state1_conc q1)) w1.
+Lemma nfa_conc_fin1 x1 w:
+  nfa_fin A1 x1 ->
+  nfa_lang A2 w ->
+  nfa_accept nfa_conc (inl _ x1) w.
 Proof.
-elim: w1 q1 => [|a w1 IHw1] q1.
-  rewrite /fin_det /fin_conc /accept /accept' /=.
-  move/andP => [] H0 H1. apply/existsP. exists (state1_conc q1). 
-  rewrite ffunE. apply/andP. split.
-    by apply/eqP.
-  by rewrite H0 H1.
-move/andP => [].
-move => H0 H1. move: (IHw1 (step1 q1 a)).
-rewrite accept'S in H0.
-rewrite /accept. rewrite H0 H1. move => H2. move: (H2 is_true_true).
-rewrite accept'S.
-apply Aut_conc_expand1. 
-move => q. rewrite 2!ffunE. move/eqP => ->. apply/existsP. 
-exists (state1_conc q1). rewrite ffunE. apply/andP. split.
-  by apply/eq_refl.
-rewrite/step_conc => /=. by apply/eq_refl.
+move => H0 /nfa_accept_lpath [] ys.
+elim: ys w x1 H0 => [|y ys IHys] [|a w] x1 H0 /andP //=.
+  by move: H0 => -> ->.
+move/andP => [] /andP [] H1 H2 H3.
+apply/existsP. exists (inr _ y).
+rewrite H0 H1 => /=.
+apply: nfa_lpath_accept.
+  apply nfa_conc_cont.
+  by eassumption.
+by rewrite last_map /nfa_fin.
 Qed.
+    
 
-
-(** We proof that the concatenation automaton accepts
-   all words accepted by the second automaton when if
-   they both start in the same state. **)
-Lemma Aut_conc_correct2' x2 w2: 
-accept' A2 x2 w2
--> accept' Aut_conc (finfun (fun x=> x == state2_conc x2)) w2.
-Proof. elim: w2 x2 => [|a w2 IHw2] x2 /=.
-  move => H0. rewrite/fin_det/fin_conc. apply/existsP. exists (state2_conc x2). apply/andP. split.
-    by rewrite ffunE.
-  by exact: H0.
-move/IHw2. apply: Aut_conc_expand1 => x. rewrite 2!ffunE. move/eqP => ->.
-apply/existsP. exists (state2_conc x2). apply/andP. split.
-  by rewrite ffunE. 
-by rewrite/step_conc => /=.
+Lemma nfa_conc_correct1 x w1 w2:
+  nfa_accept A1 x w1 ->
+  nfa_lang A2 w2 ->
+  nfa_accept nfa_conc (inl _ x) (w1 ++ w2).
+Proof. elim: w1 w2 x => [|a w1 IHw1] w2 x.
+  move => H0 /nfa_accept_lpath [] xs [] H1 H2.
+  move: (nfa_conc_cont _ _ _ H1) => H3.
+  apply/nfa_accept_cat.
+  exists [::] => /=.
+  apply: nfa_conc_fin1.
+    exact: H0.
+  apply: nfa_lpath_accept.
+    by eassumption.
+  exact: H2.
+move => /existsP [] y /andP [] H1 H2 H3 /=.
+apply/existsP. exists (inl _ y).
+rewrite H1 => /=.
+apply: IHw1.
+  exact: H2.
+exact: H3.
 Qed.
-
-(** We proof that final states of the first automaton have at
-   least all transitions of s02 in the concatenation automaton. **)
-Lemma Aut_conc_end1 x1 a:
-fin1 x1 ->
-step_det char step_conc [ffun x => x == state2_conc s02] a ===> step_det char step_conc [ffun x => x == state1_conc x1] a.
+  
+Lemma nfa_conc_correct2 X w :
+  nfa_accept nfa_conc X w ->
+  match X with
+  | inl x => exists w1, exists w2, (w == w1 ++ w2) && (nfa_accept A1 x w1) && nfa_lang A2 w2
+  | inr x => nfa_accept A2 x w
+end.
 Proof.
-rewrite /step_det /step_conc => /=. move => H0 [x|x];
-rewrite ffunE => /existsP [] x'; rewrite ffunE => /andP [] /eqP -> /=.
+elim: w X => [|a w IHw] [x|x] //=.
+    move => /andP [] H0 H1. exists [::]. exists [::].
+    simpl. by rewrite H0 H1.
+  move/existsP => [] [y|y] /andP [] H0 /IHw.
+      (* inl / inl *)
+      move => [] w1 [] w2 /andP [] /andP [] /eqP H1 H2 /= H3.
+      exists (a::w1). exists w2.
+      rewrite H1 eq_refl H3 andTb andbT.
+      apply/existsP. exists y.
+      move: H0 => /= ->. rewrite andTb.
+      exact H2.
+    (* inl / inr *)
+    move: H0 => /= /andP [] H0 H1 /= H2.
+    exists [::]. exists (a::w) => /=.
+    rewrite H0 eq_refl 2!andTb.
+    apply/existsP. exists y.
+    by rewrite H1 H2.
+  (* inr / inl  *)
+  move/existsP => [] [y|y] /andP [] H0 /IHw.
   by [].
-rewrite eq_sym ffunE => /eqP ->. apply/existsP. exists (state1_conc x1).
-rewrite ffunE eq_refl andTb. by rewrite H0 eq_refl.
+(* inr / inr *)
+move: H0 => /= H0 H1.
+apply/existsP. exists y.
+by rewrite H0 H1.
 Qed.
+  
 
-(** We proof that all words accepted by s02 are also accepted
-   by final states of the first automaton in the concatenation
-   automaton. **)
-Lemma Aut_conc_correct3' x1 w2:
-fin1 x1 ->
-accept' Aut_conc [ffun x => x == state2_conc s02] w2 ->
-accept' Aut_conc [ffun x => x == state1_conc x1] w2.
-Proof. elim: w2 x1 => [|a w2 IHw2] x1 H0 /=.
-  rewrite/fin_det/fin_conc. move/existsP => [] x /andP []. rewrite ffunE => /eqP -> /= H1.
-  apply/existsP. exists (state1_conc x1). by rewrite ffunE eq_refl andTb H0 H1.
-apply: Aut_conc_expand1. apply: Aut_conc_end1. exact: H0.
-Qed.
+End NFAOps.
 
-(** We proof that the concatenation automaton accepts
-   all words that are made up of a prefix accepted by the first automaton
-   and a suffix accepted by the second automaton. **)
-Lemma Aut_conc_correct1 x1 w1 w2: (accept' A1 x1 w1 && accept A2 w2) ->
-  accept' Aut_conc [ffun x => x == state1_conc x1] (w1 ++ w2).
-Proof. elim: w1 w2 x1 => [|a w1 IHw1] w2 x1.
-  rewrite/accept => /andP [] /= H0. rewrite/s0_conc. move/(Aut_conc_correct2').
-  rewrite/state2_conc. apply: Aut_conc_correct3'. exact: H0.
-simpl. move/IHw1. apply: Aut_conc_expand1 => x.
-rewrite /step_det /step_conc ffunE => /eqP -> /=. rewrite ffunE. apply/existsP.
-exists (state1_conc x1). by rewrite ffunE eq_refl andTb eq_refl.
-Qed.
-
-(** We proof that the concatenation automaton only accepts
-   words that can be expressed as a prefix accepted by the first automaton
-   and a suffix accepted by the second automaton. **)
-Lemma Aut_conc_correct2 w: 
-accept' Aut_conc [ffun x => x == state1_conc s01] w -> 
-exists w1, exists w2, w = w1 ++ w2 /\ accept A1 w1 && accept A2 w2.
-Proof. move: w.
-apply: last_ind => [| w a IHw ].
-  rewrite /fin_det /fin_conc => /existsP [] x /andP []. rewrite ffunE => /eqP -> /= /andP [] H0 H1.
-  exists [::]. exists [::]. rewrite/accept => /=. by rewrite H0 H1.
-case_eq (accept A1 (rcons w a)); case_eq (accept A2 [::]); move => H0 H1.
-      exists (rcons w a). exists [::]. by rewrite cats0 H0 H1.
-    case_eq (accept' Aut_conc [ffun x => x == state1_conc s01] w).
-      move/IHw => [] w1 [] w2 [] -> /andP [] H2 H3. rewrite rcons_cat.
-      case_eq (accept A2 (rcons w2 a)) => H4.
-        exists w1. exists (rcons w2 a). split.
-          by [].
-        by rewrite H2 H4.
-Admitted.  
-
-
-End Concatenation.
-
-End Operators.
+End FA.
 
 
